---
marp: true
theme: dracula
---

<!-- _class: slide__chapter -->

## Product

---

<!-- _class: slide__section -->

### $ax^2 + c = 0$

---

<!-- _class: slide__section__subtitle -->

#### Example 1

---

<!-- _class: slide__algebra -->

$$x^2 = 16$$

---

<!-- _class: slide__algebra -->

$$x^2 = 16$$

$$x = \pm 4$$

---

<!-- _class: slide__algebra -->

$$x^2 = 16$$

$$x = \pm 4$$

$$x_1 \cdot x_2 = -4 \cdot 4 = -16$$

---

<!-- _class: slide__section__subtitle -->

#### Example 2

---

<!-- _class: slide__algebra -->

$$7x^2 = 63$$

---

<!-- _class: slide__algebra -->

$$7x^2 = 63$$

$$x^2 = 9$$

---

<!-- _class: slide__algebra -->

$$7x^2 = 63$$

$$x^2 = 9$$

$$x = \pm 3$$

---

<!-- _class: slide__algebra -->

$$7x^2 = 63$$

$$x^2 = 9$$

$$x = \pm 3$$

$$x_1 = -3, x_2 = 3$$

---

<!-- _class: slide__algebra -->

$$7x^2 = 63$$

$$x^2 = 9$$

$$x = \pm 3$$

$$x_1 = -3, x_2 = 3$$

$$x_1 \cdot x_2 = -9$$

---

<!-- _class: slide__section__subtitle -->

#### Generalizing

---

<!-- _class: slide__algebra -->

$$ax^2 = c$$

---

<!-- _class: slide__algebra -->

$$ax^2 = c$$

$$x^2 = \frac{c}{a}$$

---

<!-- _class: slide__algebra -->

$$ax^2 = c$$

$$x^2 = \frac{c}{a}$$

$$x = \pm \sqrt{\frac{c}{a}}$$

---

<!-- _class: slide__algebra -->

$$ax^2 = c$$

$$x^2 = \frac{c}{a}$$

$$x = \pm \sqrt{\frac{c}{a}}$$

$$x_1 \cdot x_2 = -\sqrt{\frac{c}{a}} \cdot \sqrt{\frac{c}{a}}$$

---

<!-- _class: slide__algebra -->

$$ax^2 = c$$

$$x^2 = \frac{c}{a}$$

$$x = \pm \sqrt{\frac{c}{a}}$$

$$x_1 \cdot x_2 = -\sqrt{\frac{c}{a}} \cdot \sqrt{\frac{c}{a}}$$

$$x_1 \cdot x_2 = -\frac{c}{a}$$

---

<!-- _class: slide__section -->

### $$a(x-h)^2 + k = 0$$

---

<!-- _class: slide__section__subtitle -->

#### Example 1

---

<!-- _class: slide__algebra -->

$$(x-5)^2 = 16$$

---

<!-- _class: slide__algebra -->

$$(x-5)^2 = 16$$

$$x - 5 = \pm 4$$

---

<!-- _class: slide__algebra -->

$$(x-5)^2 = 16$$

$$x - 5 = \pm 4$$

$$x = 5 \pm 4$$

---

<!-- _class: slide__algebra -->

$$(x-5)^2 = 16$$

$$x - 5 = \pm 4$$

$$x = 5 \pm 4$$

$$x_1 = 5 + 4$$

---

<!-- _class: slide__algebra -->

$$(x-5)^2 = 16$$

$$x - 5 = \pm 4$$

$$x = 5 \pm 4$$

$$x_1 = 5 + 4$$

$$x_2 = 5 - 4$$

---

<!-- _class: slide__algebra -->

$$(x-5)^2 = 16$$

$$x - 5 = \pm 4$$

$$x = 5 \pm 4$$

$$x_1 = 5 + 4$$

$$x_2 = 5 - 4$$

$$x_1 \cdot x_2 = (5 + 4)(5 - 4) = 5^2 - 4^2$$

---

<!-- _class: slide__algebra -->

$$(x-5)^2 = 16$$

$$x - 5 = \pm 4$$

$$x = 5 \pm 4$$

$$x_1 = 5 + 4$$

$$x_2 = 5 - 4$$

$$x_1 \cdot x_2 = (5 + 4)(5 - 4) = 5^2 - 4^2$$

$$x_1 \cdot x_2 = 25 - 16 = 9$$

---

<!-- _class: slide__algebra -->

$$(x - 2)^2 = 7$$

---

<!-- _class: slide__algebra -->

$$(x - 2)^2 = 7$$

$$x - 2 = \pm \sqrt{7}$$

---

<!-- _class: slide__algebra -->

$$(x - 2)^2 = 7$$

$$x - 2 = \pm \sqrt{7}$$

$$x = 2 \pm \sqrt{7}$$

---

<!-- _class: slide__algebra -->

$$(x - 2)^2 = 7$$

$$x - 2 = \pm \sqrt{7}$$

$$x = 2 \pm \sqrt{7}$$

$$x_1 \cdot x_2 = (2 - \sqrt{7})(2 + \sqrt{7}) = 2^2 - 7$$

---

<!-- _class: slide__algebra -->

$$(x - 2)^2 = 7$$

$$x - 2 = \pm \sqrt{7}$$

$$x = 2 \pm \sqrt{7}$$

$$x_1 \cdot x_2 = (2 - \sqrt{7})(2 + \sqrt{7}) = 2^2 - 7$$

$$x_1 \cdot x_2 = h^2 + k$$

---

<!-- _class: slide__section -->

## $ax^2 + bx + c = 0$

---

<!-- _class: slide__section__subtitle -->

#### Generalizing

---

<!-- _class: slide__algebra -->

$$x = \frac{-b}{2a} \pm \frac{\sqrt{b^2 - 4ac}}{2a}$$

---

<!-- _class: slide__algebra -->

$$x = \frac{-b}{2a} \pm \frac{\sqrt{b^2 - 4ac}}{2a}$$

$$x_1 \cdot x_2 = \left( -\frac{b}{2a} - \frac{\sqrt{b^2 - 4ac}}{2a} \right) \left( -\frac{b}{2a} + \frac{\sqrt{b^2 - 4ac}}{2a} \right)$$

---

<!-- _class: slide__algebra -->

$$x = \frac{-b}{2a} \pm \frac{\sqrt{b^2 - 4ac}}{2a}$$

$$x_1 \cdot x_2 = \left( -\frac{b}{2a} - \frac{\sqrt{b^2 - 4ac}}{2a} \right) \left( -\frac{b}{2a} + \frac{\sqrt{b^2 - 4ac}}{2a} \right)$$

$$x_1 \cdot x_2 = \left( -\frac{b}{2a} \right)^2 - \left( \frac{\sqrt{b^2 - 4ac}}{2a} \right)^2$$

---

<!-- _class: slide__algebra -->

$$x = \frac{-b}{2a} \pm \frac{\sqrt{b^2 - 4ac}}{2a}$$

$$x_1 \cdot x_2 = \left( -\frac{b}{2a} - \frac{\sqrt{b^2 - 4ac}}{2a} \right) \left( -\frac{b}{2a} + \frac{\sqrt{b^2 - 4ac}}{2a} \right)$$

$$x_1 \cdot x_2 = \left( -\frac{b}{2a} \right)^2 - \left( \frac{\sqrt{b^2 - 4ac}}{2a} \right)^2$$

$$x_1 \cdot x_2 = \frac{b^2}{(2a)^2} - \frac{b^2 - 4ac}{(2a)^2}$$

---

<!-- _class: slide__algebra -->

$$x_1 \cdot x_2 = \frac{b^2}{(2a)^2} - \frac{b^2 - 4ac}{(2a)^2}$$

---

<!-- _class: slide__algebra -->

$$x_1 \cdot x_2 = \frac{b^2}{(2a)^2} - \frac{b^2 - 4ac}{(2a)^2}$$

$$x_1 \cdot x_2 = \frac{b^2 - (b^2 - 4ac)}{4a^2}$$

---

<!-- _class: slide__algebra -->

$$x_1 \cdot x_2 = \frac{b^2}{(2a)^2} - \frac{b^2 - 4ac}{(2a)^2}$$

$$x_1 \cdot x_2 = \frac{b^2 - (b^2 - 4ac)}{4a^2}$$

$$x_1 \cdot x_2 = \frac{4ac}{4a^2}$$

---

<!-- _class: slide__algebra -->

$$x_1 \cdot x_2 = \frac{b^2}{(2a)^2} - \frac{b^2 - 4ac}{(2a)^2}$$

$$x_1 \cdot x_2 = \frac{b^2 - (b^2 - 4ac)}{4a^2}$$

$$x_1 \cdot x_2 = \frac{4ac}{4a^2}$$

$$x_1 \cdot x_2 = \frac{c}{a}$$

---

<!-- _class: slide__section__subtitle -->

#### Generalizing

---

<!-- _class: slide__algebra -->

$$a(x - p)(x - q) = 0$$

---

<!-- _class: slide__algebra -->

$$a(x - p)(x - q) = 0$$

$$a(x^2 - px - qx + pq) = 0$$

---

<!-- _class: slide__algebra -->

$$a(x - p)(x - q) = 0$$

$$a(x^2 - px - qx + pq) = 0$$

$$ax^2 - a(p + q)x + apq = 0$$

---

<!-- _class: slide__algebra -->

$$a(x - p)(x - q) = 0$$

$$a(x^2 - px - qx + pq) = 0$$

$$ax^2 - a(p + q)x + apq = 0$$

$$ax^2 + bx + c = 0$$

---

<!-- _class: slide__algebra -->

$$a(x - p)(x - q) = 0$$

$$a(x^2 - px - qx + pq) = 0$$

$$ax^2 - a(p + q)x + apq = 0$$

$$ax^2 + bx + c = 0$$

$$b = -a(p + q)$$

---

<!-- _class: slide__algebra -->

$$a(x - p)(x - q) = 0$$

$$a(x^2 - px - qx + pq) = 0$$

$$ax^2 - a(p + q)x + apq = 0$$

$$ax^2 + bx + c = 0$$

$$b = -a(p + q)$$

$$c = apq$$

---

<!-- _class: slide__algebra -->

$$a(x - p)(x - q) = 0$$

$$a(x^2 - px - qx + pq) = 0$$

$$ax^2 - a(p + q)x + apq = 0$$

$$ax^2 + bx + c = 0$$

$$b = -a(p + q)$$

$$c = apq$$

$$pq = \frac{c}{a}$$

---
