---
marp: true
theme: dracula
---

<!-- _class: slide__chapter -->

## Sum

---

<!-- _class: slide__section -->

### $ax^2 + c = 0$

---

<!-- _class: slide__section__subtitle -->

#### Example 1

---

<!-- _class: slide__algebra -->

$$x^2 = 16$$

---

<!-- _class: slide__algebra -->

$$x^2 = 16$$

$$x = \pm 4$$

---

<!-- _class: slide__algebra -->

$$x^2 = 16$$

$$x = \pm 4$$

$$x_1 = -4, x_2 = 4$$

---

<!-- _class: slide__algebra -->

$$x^2 = 16$$

$$x = \pm 4$$

$$x_1 = -4, x_2 = 4$$

$$x_1 + x_2 = 0$$

---

<!-- _class: slide__section__subtitle -->

#### Example 2

---

<!-- _class: slide__algebra -->

$$5x^2 = 125$$

---

<!-- _class: slide__algebra -->

$$5x^2 = 125$$

$$x^2 = 25$$

---

<!-- _class: slide__algebra -->

$$5x^2 = 125$$

$$x^2 = 25$$

$$x = \pm 5$$

---

<!-- _class: slide__algebra -->

$$5x^2 = 125$$

$$x^2 = 25$$

$$x = \pm 5$$

$$x_1 = -5, x_2 = 5$$

---

<!-- _class: slide__algebra -->

$$5x^2 = 125$$

$$x^2 = 25$$

$$x = \pm 5$$

$$x_1 = -5, x_2 = 5$$

$$x_1 + x_2 = 0$$

---

<!-- _class: slide__section__subtitle -->

##### Generalizing

---

<!-- _class: slide__algebra -->

$$ax^2 = c$$

---

$$ax^2 = c$$

$$x^2 = \frac{c}{a}$$

---

$$ax^2 = c$$

$$x^2 = \frac{c}{a}$$

$$x = \pm \sqrt{\frac{c}{a}}$$

---

$$ax^2 = c$$

$$x^2 = \frac{c}{a}$$

$$x = \pm \sqrt{\frac{c}{a}}$$

$$x_1 = -\sqrt{\frac{c}{a}}, x_2 = \sqrt{\frac{c}{a}}$$

---

$$ax^2 = c$$

$$x^2 = \frac{c}{a}$$

$$x = \pm \sqrt{\frac{c}{a}}$$

$$x_1 = -\sqrt{\frac{c}{a}}, x_2 = \sqrt{\frac{c}{a}}$$

$$x_1 + x_2 = 0$$

---

<!-- _class: slide__algebra -->

$$ax^2 + c = 0$$

---

<!-- _class: slide__algebra -->

$$ax^2 + c = 0$$

$$ax^2 = -c$$

---

<!-- _class: slide__algebra -->

$$ax^2 + c = 0$$

$$ax^2 = -c$$

$$x^2 = -\frac{c}{a}$$

---

<!-- _class: slide__algebra -->

$$ax^2 + c = 0$$

$$ax^2 = -c$$

$$x^2 = -\frac{c}{a}$$

$$x = \pm \sqrt{\frac{-c}{a}}$$

---

<!-- _class: slide__algebra -->

$$ax^2 + c = 0$$

$$ax^2 = -c$$

$$x^2 = -\frac{c}{a}$$

$$x = \pm \sqrt{\frac{-c}{a}}$$

$$x_1 = -\sqrt{\frac{-c}{a}}, x_2 = \sqrt{\frac{-c}{a}}$$

---

$$ax^2 + c = 0$$

$$ax^2 = -c$$

$$x^2 = -\frac{c}{a}$$

$$x = \pm \sqrt{\frac{-c}{a}}$$

$$x_1 = -\sqrt{\frac{-c}{a}}, x_2 = \sqrt{\frac{-c}{a}}$$

$$x_1 + x_2 = 0$$

---

<!-- _class: slide__section -->

### $a(x-h)^2 + k = 0$

---

<!-- _class: slide__section__subtitle -->

#### Example 1

---

<!-- _class: slide__algebra -->

$$(x-1)^2 = 9$$

---

<!-- _class: slide__algebra -->

$$(x-1)^2 = 9$$

$$x - 1 = \pm 3$$

---

<!-- _class: slide__algebra -->

$$(x-1)^2 = 9$$

$$x - 1 = \pm 3$$

$$x = 1 \pm 3$$

---

<!-- _class: slide__algebra -->

$$(x-1)^2 = 9$$

$$x - 1 = \pm 3$$

$$x = 1 \pm 3$$

$$x_1 = 1 - 3$$

---

<!-- _class: slide__algebra -->

$$(x-1)^2 = 9$$

$$x - 1 = \pm 3$$

$$x = 1 \pm 3$$

$$x_1 = 1 - 3$$

$$x_2 = 1 + 3$$

---

<!-- _class: slide__algebra -->

$$(x-1)^2 = 9$$

$$x - 1 = \pm 3$$

$$x = 1 \pm 3$$

$$x_1 = 1 - 3$$

$$x_2 = 1 + 3$$

$$x_1 + x_2 = 1 - 3 + 1 + 3$$

---

<!-- _class: slide__algebra -->

$$(x-1)^2 = 9$$

$$x - 1 = \pm 3$$

$$x = 1 \pm 3$$

$$x_1 = 1 - 3$$

$$x_2 = 1 + 3$$

$$x_1 + x_2 = 1 - 3 + 1 + 3$$

$$x_1 + x_2 = 2$$

---

<!-- _class: slide__section__subtitle -->

#### Example 2

---

<!-- _class: slide__algebra -->

$$5(x-13)^2 = 125$$

---

<!-- _class: slide__algebra -->

$$5(x-13)^2 = 125$$

$$(x-13)^2 = 25$$

---

<!-- _class: slide__algebra -->

$$5(x-13)^2 = 125$$

$$(x-13)^2 = 25$$

$$x - 13 = \pm 5$$

---

<!-- _class: slide__algebra -->

$$5(x-13)^2 = 125$$

$$(x-13)^2 = 25$$

$$x - 13 = \pm 5$$

$$x = 13 \pm 5$$

---

<!-- _class: slide__algebra -->

$$5(x-13)^2 = 125$$

$$(x-13)^2 = 25$$

$$x - 13 = \pm 5$$

$$x = 13 \pm 5$$

$$x_1 = 13 - 5, x_2 = 13 + 5$$

---

<!-- _class: slide__algebra -->

$$5(x-13)^2 = 125$$

$$(x-13)^2 = 25$$

$$x - 13 = \pm 5$$

$$x = 13 \pm 5$$

$$x_1 = 13 - 5, x_2 = 13 + 5$$

$$x_1 + x_2 = 13 - 5 + 13 + 5$$

---

<!-- _class: slide__algebra -->

$$5(x-13)^2 = 125$$

$$(x-13)^2 = 25$$

$$x - 13 = \pm 5$$

$$x = 13 \pm 5$$

$$x_1 = 13 - 5, x_2 = 13 + 5$$

$$x_1 + x_2 = 13 - 5 + 13 + 5$$

$$x_1 + x_2 = 26$$

---

<!-- _class: slide__section__subtitle -->

##### Generalizing

---

<!-- _class: slide__algebra -->

$$a(x-h)^2 + k = 0$$

---

<!-- _class: slide__algebra -->

$$a(x-h)^2 + k = 0$$

$$a(x-h)^2 = -k$$

---

<!-- _class: slide__algebra -->

$$a(x-h)^2 + k = 0$$

$$a(x-h)^2 = -k$$

$$(x-h)^2 = -\frac{k}{a}$$

---

<!-- _class: slide__algebra -->

$$a(x-h)^2 + k = 0$$

$$a(x-h)^2 = -k$$

$$(x-h)^2 = -\frac{k}{a}$$

$$x - h = \pm \sqrt{-\frac{k}{a}}$$

---

<!-- _class: slide__algebra -->

$$a(x-h)^2 + k = 0$$

$$a(x-h)^2 = -k$$

$$(x-h)^2 = -\frac{k}{a}$$

$$x - h = \pm \sqrt{-\frac{k}{a}}$$

$$x = h \pm \sqrt{-\frac{k}{a}}$$

---

<!-- _class: slide__algebra -->

$$x = h \pm \sqrt{-\frac{k}{a}}$$

---

<!-- _class: slide__algebra -->

$$x = h \pm \sqrt{-\frac{k}{a}}$$

$$x_1 = h - \sqrt{-\frac{k}{a}}$$

---

<!-- _class: slide__algebra -->

$$x = h \pm \sqrt{-\frac{k}{a}}$$

$$x_1 = h - \sqrt{-\frac{k}{a}}$$

$$x_2 = h + \sqrt{-\frac{k}{a}}$$

---

<!-- _class: slide__algebra -->

$$x = h \pm \sqrt{-\frac{k}{a}}$$

$$x_1 = h - \sqrt{-\frac{k}{a}}$$

$$x_2 = h + \sqrt{-\frac{k}{a}}$$

$$x_1 + x_2 = 2h$$

---

<!-- _class: slide__section -->

### $ax^2 + bx + c = 0$

---

<!-- _class: slide__section__subtitle -->

#### Example 1

---

<!-- _class: slide__algebra -->

$$x^2 + 8x + 15 = 0$$

---

<!-- _class: slide__algebra -->

$$x^2 + 8x + 15 = 0$$

$$(x + 3)(x + 5) = 0$$

---

<!-- _class: slide__algebra -->

$$x^2 + 8x + 15 = 0$$

$$(x + 3)(x + 5) = 0$$

$$x_1 = -3, x_2 = -5$$

---

<!-- _class: slide__algebra -->

$$x^2 + 8x + 15 = 0$$

$$(x + 3)(x + 5) = 0$$

$$x_1 = -3, x_2 = -5$$

$$x_1 + x_2 = -8$$

---

<!-- _class: slide__section__subtitle -->

#### Example 2

---

<!-- _class: slide__algebra -->

$$x^2 - 7x - 30 = 0$$

---

<!-- _class: slide__algebra -->

$$x^2 - 7x - 30 = 0$$

$$(x - 10)(x + 3) = 0$$

---

<!-- _class: slide__algebra -->

$$x^2 - 7x - 30 = 0$$

$$(x - 10)(x + 3) = 0$$

$$x_1 = -3$$

---

<!-- _class: slide__algebra -->

$$x^2 - 7x - 30 = 0$$

$$(x - 10)(x + 3) = 0$$

$$x_1 = -3$$

$$x_2 = 10$$

---

<!-- _class: slide__algebra -->

$$x^2 - 7x - 30 = 0$$

$$(x - 10)(x + 3) = 0$$

$$x_1 = -3$$

$$x_2 = 10$$

$$x_1 + x_2 = 7$$

---

<!-- _class: slide__section__subtitle -->

#### Generalizing

---

<!-- _class: slide__algebra -->

$$a(x-p)(x-q) = 0$$

---

<!-- _class: slide__algebra -->

$$a(x-p)(x-q) = 0$$

$$a(x^2 - px - qx + pq) = 0$$

---

<!-- _class: slide__algebra -->

$$a(x-p)(x-q) = 0$$

$$a(x^2 - px - qx + pq) = 0$$

$$a(x^2 - (p+q)x + pq) = 0$$

---

<!-- _class: slide__algebra -->

$$a(x-p)(x-q) = 0$$

$$a(x^2 - px - qx + pq) = 0$$

$$a(x^2 - (p+q)x + pq) = 0$$

$$ax^2 - a(p+q)x + apq = 0$$

---

<!-- _class: slide__algebra -->

$$a(x-p)(x-q) = 0$$

$$a(x^2 - px - qx + pq) = 0$$

$$a(x^2 - (p+q)x + pq) = 0$$

$$ax^2 - a(p+q)x + apq = 0$$

$$ax^2 + bx + c = 0$$

---

<!-- _class: slide__algebra -->

$$a(x-p)(x-q) = 0$$

$$a(x^2 - px - qx + pq) = 0$$

$$a(x^2 - (p+q)x + pq) = 0$$

$$ax^2 - a(p+q)x + apq = 0$$

$$ax^2 + bx + c = 0$$

$$-a(p+q) = b$$

---

<!-- _class: slide__algebra -->

$$a(x-p)(x-q) = 0$$

$$a(x^2 - px - qx + pq) = 0$$

$$a(x^2 - (p+q)x + pq) = 0$$

$$ax^2 - a(p+q)x + apq = 0$$

$$ax^2 + bx + c = 0$$

$$-a(p+q) = b$$

$$p + q = -\frac{b}{a}$$

---

<!-- _class: slide__algebra -->

$$ax^2 + bx + c = 0$$

---

<!-- _class: slide__algebra -->

$$ax^2 + bx + c = 0$$

$$x = \frac{-b}{2a} \pm \frac{\sqrt{b^2 - 4ac}}{2a}$$

---

<!-- _class: slide__algebra -->

$$ax^2 + bx + c = 0$$

$$x = \frac{-b}{2a} \pm \frac{\sqrt{b^2 - 4ac}}{2a}$$

$$x_1 = \frac{-b}{2a} - \frac{\sqrt{b^2 - 4ac}}{2a}$$

---

<!-- _class: slide__algebra -->

$$ax^2 + bx + c = 0$$

$$x = \frac{-b}{2a} \pm \frac{\sqrt{b^2 - 4ac}}{2a}$$

$$x_1 = \frac{-b}{2a} - \frac{\sqrt{b^2 - 4ac}}{2a}$$

$$x_2 = \frac{-b}{2a} + \frac{\sqrt{b^2 - 4ac}}{2a}$$

---

<!-- _class: slide__algebra -->

$$ax^2 + bx + c = 0$$

$$x = \frac{-b}{2a} \pm \frac{\sqrt{b^2 - 4ac}}{2a}$$

$$x_1 = \frac{-b}{2a} - \frac{\sqrt{b^2 - 4ac}}{2a}$$

$$x_2 = \frac{-b}{2a} + \frac{\sqrt{b^2 - 4ac}}{2a}$$

$$x_1 + x_2 = \frac{-b}{2a} + \frac{\sqrt{b^2 - 4ac}}{2a} + \frac{-b}{2a} - \frac{\sqrt{b^2 - 4ac}}{2a}$$

---

<!-- _class: slide__algebra -->

$$x_1 + x_2 = \frac{-b}{2a} + \frac{\sqrt{b^2 - 4ac}}{2a} + \frac{-b}{2a} - \frac{\sqrt{b^2 - 4ac}}{2a}$$

---

<!-- _class: slide__algebra -->

$$x_1 + x_2 = \frac{-b}{2a} + \frac{\sqrt{b^2 - 4ac}}{2a} + \frac{-b}{2a} - \frac{\sqrt{b^2 - 4ac}}{2a}$$

$$x_1 + x_2 = \frac{-b}{2a} + \cancel{\frac{ \sqrt{b^2 - 4ac}}{2a} } + \frac{-b}{2a} \cancel{ -\frac{\sqrt{b^2 - 4ac}}{2a} }$$

---

<!-- _class: slide__algebra -->

$$x_1 + x_2 = \frac{-b}{2a} + \frac{\sqrt{b^2 - 4ac}}{2a} + \frac{-b}{2a} - \frac{\sqrt{b^2 - 4ac}}{2a}$$

$$x_1 + x_2 = \frac{-b}{2a} + \cancel{\frac{ \sqrt{b^2 - 4ac}}{2a} } + \frac{-b}{2a} \cancel{ -\frac{\sqrt{b^2 - 4ac}}{2a} }$$

$$x_1 + x_2 = \frac{-b}{2a}  + \frac{-b}{2a} $$

---

<!-- _class: slide__algebra -->

$$x_1 + x_2 = \frac{-b}{2a} + \frac{\sqrt{b^2 - 4ac}}{2a} + \frac{-b}{2a} - \frac{\sqrt{b^2 - 4ac}}{2a}$$

$$x_1 + x_2 = \frac{-b}{2a} + \cancel{\frac{ \sqrt{b^2 - 4ac}}{2a} } + \frac{-b}{2a} \cancel{ -\frac{\sqrt{b^2 - 4ac}}{2a} }$$

$$x_1 + x_2 = \frac{-b}{2a}  + \frac{-b}{2a} $$

$$x_1 + x_2 = \frac{-2b}{2a}$$

---

<!-- _class: slide__algebra -->

$$x_1 + x_2 = \frac{-b}{2a} + \frac{\sqrt{b^2 - 4ac}}{2a} + \frac{-b}{2a} - \frac{\sqrt{b^2 - 4ac}}{2a}$$

$$x_1 + x_2 = \frac{-b}{2a} + \cancel{\frac{ \sqrt{b^2 - 4ac}}{2a} } + \frac{-b}{2a} \cancel{ -\frac{\sqrt{b^2 - 4ac}}{2a} }$$

$$x_1 + x_2 = \frac{-b}{2a}  + \frac{-b}{2a} $$

$$x_1 + x_2 = \frac{-2b}{2a}$$

$$x_1 + x_2 = - \frac{b}{a}$$

---

And if you're not used to seeing the quadratic formula like this, that's because the educational system has failed you. For the tiny price of repeating the $2a$, this otherwise mysterious beast of a formula suddenly opens itself up to us.

For this:

$$-\frac{b}{2a}$$

is the axis of symmetry, and this:

$$\pm \frac{\sqrt{b^2 - 4ac}}{2a}$$

is the number of steps we walk to get to the solutions:

$$+\frac{\sqrt{b^2 - 4ac}}{2a}$$

steps to the right and

$$-\frac{\sqrt{b^2 - 4ac}}{2a}$$

steps to the left from the axis of symmetry:

$$-\frac{b}{2a}$$

And we know that if we double the axis of symmetry, we get the sum of the solutions:

$$2 \cdot \left( -\frac{b}{2a} \right) = -\frac{b}{a}$$
